src/common/Nemonuri.Bijective.IndexMap.fst
@@ -3,10 +3,9 @@ module Nemonuri.Bijective.IndexMap
 module I = FStar.IntegerIntervals
 module ISet = Nemonuri.IndexSet
 module IMap = Nemonuri.IndexMap
-//open FStar.Bijection { ( =~ ) }
-//module B = FStar.Bijection
 module Seq = FStar.Seq.Base
 module List = FStar.List.Tot
+module B = FStar.Bijection
 
 let bijective_index_map_predicate (#data_t:eqtype) (m:IMap.t data_t) =
   m |> IMap.to_seq |> Seq.seq_to_list |> List.noRepeats
@@ -15,4 +14,20 @@ type t (data_t:eqtype) = x:IMap.t data_t{bijective_index_map_predicate x}
 
 //let index_of 
 
-//let lemma_bijective_index_map 
+//let lemma_bijective_index_map #data_t (m:t data_t)
+//  : Lemma
+
+
+
+
+type bijection_t #data_t (m:t data_t) = B.bijection (IMap.key_t m) (IMap.contained_data_t m)
+
+
+
+(*
+let to_bijection #data_t (m:t data_t)
+  : Tot (bijection_t m) =
+  {
+    right = 
+  }
+*)
